pulse/pulse2rust/src/Pulse2Rust.fst
@@ -35,7 +35,10 @@ let tyvar_of (s:string) : string =
 //
 // Pulse has variable _'n, which are not valid in Rust
 //
-let varname (s:string) : string = replace_char s '\'' '_'
+let varname (s:string) : string =
+  if s = "uu___"
+  then "_"
+  else replace_char s '\'' '_'
 
 let fail (s:string) =
   failwith (format1 "Pulse to Rust extraction failed: %s" s)
@@ -459,14 +462,18 @@ and extract_mlexpr_to_stmts (g:env) (e:S.mlexpr) : list stmt =
   let is_assign (e:S.mlexpr) =
     match e.expr with
     | S.MLE_App ({expr=S.MLE_TApp ({expr=S.MLE_Name p}, [_])}, _) ->
-      S.string_of_mlpath p = "Pulse.Lib.Reference.op_Colon_Equals"
+      let p = S.string_of_mlpath p in
+      p = "Pulse.Lib.Reference.op_Colon_Equals"
+    // | S.MLE_App ({expr=S.MLE_Name p}, _) ->
+    //   let p = S.string_of_mlpath p in
+    //   p = "Pulse.Lib.Reference.write_atomic"
     | _ -> false
   in
 
   match e.expr with
-  | S.MLE_Const S.MLC_Unit -> []
-  | S.MLE_Var x -> [Stmt_expr (mk_expr_path_singl (varname x))]
-  | S.MLE_Name p -> [Stmt_expr (mk_expr_path_singl (S.mlpath_to_string p))]
+  // | S.MLE_Const S.MLC_Unit -> []
+  // | S.MLE_Var x -> [Stmt_expr (mk_expr_path_singl (varname x))]
+  // | S.MLE_Name p -> [Stmt_expr (mk_expr_path_singl (S.mlpath_to_string p))]
 
   | S.MLE_Let ((S.NonRec, [{mllb_def=e1}]), e2)
     when is_assign e1 ->
@@ -474,13 +481,18 @@ and extract_mlexpr_to_stmts (g:env) (e:S.mlexpr) : list stmt =
 
   | S.MLE_Let ((S.NonRec, [lb]), e) ->
     let is_mut, ty, init = lb_init_and_def g lb in
-    let s = mk_local_stmt lb.mllb_name is_mut init in
+    let s = mk_local_stmt (varname lb.mllb_name) is_mut init in
     s::(extract_mlexpr_to_stmts (push_local g lb.mllb_name ty is_mut) e)
 
   | S.MLE_App ({ expr=S.MLE_TApp ({ expr=S.MLE_Name p }, _) }, _)
     when S.string_of_mlpath p = "failwith" ->
     [Stmt_expr (mk_call (mk_expr_path_singl panic_fn) [])]
-  | _ -> fail_nyi (format1 "mlexpr_to_stmt  %s" (S.mlexpr_to_string e))
+
+  | _ -> [Stmt_expr (extract_mlexpr g e)]
+
+  // | _ -> extra
+
+  // | _ -> fail_nyi (format1 "mlexpr_to_stmt  %s" (S.mlexpr_to_string e))
 
 and extract_mlbranch_to_arm (g:env) ((pat, pat_guard, body):S.mlbranch) : arm =
   match pat_guard with
